experiments/param/GhostSnapshot1.fst
@@ -6,8 +6,10 @@ module GhostRefParam2
 noeq
 type erased_ix = {
   m : bool -> Type0 -> Type0;
+  erased : Type0 -> Type0;
 
-  hide : t:_ -> t -> m true t;
+  hide : t:_ -> t -> erased t;
+  reveal : t:_ -> erased t -> m true t;
   
   subt : t:_ -> m false t -> m true t;
   ret : a:_ -> a -> m false a;
@@ -27,7 +29,7 @@ let bool_param = param_of_eqtype bool
 
 %splice[erased_ix_param; Mkerased_ix_param] (paramd (`%erased_ix))
 
-%splice[__proj__Mkerased_ix__item__m_param] (paramd (`%__proj__Mkerased_ix__item__m))
+%splice[__proj__Mkerased_ix__item__erased_param] (paramd (`%__proj__Mkerased_ix__item__erased))
 
 // since an erased_ix provides no way to extract an erased or an m, they are
 // all related to each other
@@ -43,7 +45,9 @@ let bool_param = param_of_eqtype bool
 
 let erased_ix_irrel : erased_ix = {
   m = (fun b t -> if b then unit else t);
+  erased = (fun _ -> unit);
   hide = (fun _ _ -> ());
+  reveal = (fun _ _ -> ());
   subt = (fun _ _ -> ());
   ret = (fun _ x -> x);
   bind = (fun a b f x k -> if f then () else k x);
@@ -57,7 +61,9 @@ let erased_ix_irrel_param : erased_ix_param erased_ix_irrel erased_ix_irrel =
   let ix2 = ix1 in
    Mkerased_ix_param
      ix1.m      ix2.m       (fun b1 b2 bR t1 t2 tR m1 m2 -> if not b1 then (tR m1 m2) else True)
+     ix1.erased ix2.erased  (fun t1 t2 tR e1 e2 -> squash True)
      ix1.hide   ix2.hide    (fun t1 t2 tR x1 x2 xR -> ())
+     ix1.reveal ix2.reveal  (fun t1 t2 tR e1 e2 eR -> ())
      ix1.subt   ix2.subt    (fun t1 t2 tR e1 e2 eR -> ())
      ix1.ret    ix2.ret     (fun a1 a2 aR x1 x2 xR -> xR)
      ix1.bind   ix2.bind    (fun a1 a2 aR b1 b2 bR f1 f2 fR c1 c2 cR k1 k2 kR ->
@@ -75,10 +81,10 @@ let erased_ix_irrel_param : erased_ix_param erased_ix_irrel erased_ix_irrel =
 // and match on it, how can we model that? This is one attempt.. maybe
 // it can instead be inside of the erased_ix type, alongside a field
 // stating that m f phi ==> phi, or something akin to that.
-assume val reveal2 : (#ix:erased_ix) -> #b:Type0 -> ix.m true b -> GTot b
-assume val reveal2_inv : (#ix:erased_ix) -> #b:Type0 -> e:(ix.m true b) -> v:b -> Lemma (requires e == ix.hide b v) (ensures reveal2 e == v)
+assume val reveal2 : (#ix:erased_ix) -> #b:Type0 -> ix.erased b -> GTot b
+assume val reveal2_inv : (#ix:erased_ix) -> #b:Type0 -> e:(ix.erased b) -> v:b -> Lemma (requires e == ix.hide b v) (ensures reveal2 e == v)
 
-let ty = (ix : erased_ix) -> (b : ix.m true bool) -> x:int -> y:int{if reveal2 b then y==x else True}
+let ty = (ix : erased_ix) -> (b : ix.erased bool) -> x:int -> y:int{if reveal2 b then y==x else True}
 
 #set-options "--print_universes"
 
@@ -90,25 +96,26 @@ let ty_param (f0 f1 : ty) : Type u#1 =
     ix0: erased_ix ->
     ix1: erased_ix ->
     ixR: erased_ix_param ix0 ix1 ->
-    b0: Mkerased_ix?.m ix0 true Prims.bool ->
-    b1: Mkerased_ix?.m ix1 true Prims.bool ->
-    bR: Mkerased_ix?.m_param ix0 ix1 ixR true true () bool bool bool_param b0 b1 ->
+    b0: Mkerased_ix?.erased ix0 Prims.bool ->
+    b1: Mkerased_ix?.erased ix1 Prims.bool ->
+    bR: Mkerased_ix?.erased_param ix0 ix1 ixR bool bool bool_param b0 b1 ->
     x0: Prims.int -> x1: Prims.int -> xR: int_param x0 x1 ->
     int_param (f0 ix0 b0 x0) (f1 ix1 b1 x1)
 
 let thm
   (f : ty)
   (f_param : ty_param f f)
-: Lemma (forall b x. f erased_ix_irrel b x == x)
+  (ix : erased_ix)
+  (ix_param : erased_ix_param ix ix)
+: Lemma (forall b x. f ix b x == x)
 =
-  let aux (b : erased_ix_irrel.m true bool) x : Lemma (f erased_ix_irrel b x == x) =
-    //assert (erased_ix_irrel_param.m_param true true () intin
-    f_param erased_ix_irrel erased_ix_irrel erased_ix_irrel_param
+  let aux (b : ix.erased bool) x : Lemma (f ix b x == x) =
+    f_param ix ix ix_param
             
-            b  (erased_ix_irrel.hide _ true) ()
+            b  (ix.hide _ true) ()
             x  x ();
-    assert (f erased_ix_irrel b x == f erased_ix_irrel (erased_ix_irrel.hide _ true) x);
-    reveal2_inv (erased_ix_irrel.hide _ true) true;
+    assert (f ix b x == f ix (ix.hide _ true) x);
+    reveal2_inv (ix.hide _ true) true;
     ()
   in
   Classical.forall_intro_3 aux
